Regex/Regular/Anchor.lean
@@ -12,7 +12,7 @@ inductive CRegularAnchor : Regex α → Type u where
   | unit c : CRegularAnchor (unit c)
   | concat {q} {r} : CRegularAnchor q → CRegularAnchor r → CRegularAnchor (concat q r)
   | or {q} {r} : CRegularAnchor q → CRegularAnchor r → CRegularAnchor (or q r)
-  | star t {r} : CRegularAnchor r → CRegularAnchor (star t r)
+  | star {r} : CRegularAnchor r → CRegularAnchor (star r)
   | start : CRegularAnchor start
   | end' : CRegularAnchor end'
   | capture n {r} : CRegularAnchor r → CRegularAnchor (capture n r)
@@ -25,6 +25,26 @@ def regex {r : Regex α} (hr : r.CRegularAnchor) := r
 omit deq in
 @[simp] theorem regex_eq {r : Regex α} (hr : r.CRegularAnchor) : hr.regex = r := rfl
 
+def cTerminates {r : Regex α} (hr : r.CRegularAnchor)
+    : r.CTerminates := match hr with
+  | bot => CTerminates.bot
+  | empty => CTerminates.empty
+  | unit _ => CTerminates.unit _
+  | concat qt rt => CTerminates.concat qt.cTerminates rt.cTerminates
+  | or qt rt => CTerminates.or qt.cTerminates rt.cTerminates
+  | star rt => CTerminates.star rt.cTerminates
+  | start => CTerminates.start
+  | end' => CTerminates.end'
+  | capture n rt => CTerminates.capture n rt.cTerminates
+
+theorem allTerminates {r : Regex α} (hr : r.CRegularAnchor) :
+  r.AllTerminates := hr.cTerminates.allTerminates
+
+theorem terminatesEquiv {q r : Regex α}
+    (hq : q.CRegularAnchor) (hr : r.CRegularAnchor) : q ≃ᵗᵉ r :=
+  fun _ _ _ ↦
+    ⟨fun _ ↦ hr.allTerminates _ _ _, fun _ ↦ hq.allTerminates _ _ _⟩
+
 /-- Get a regex that's language-equivalent to this regex, but doesn't
 have any start anchors, assuming that `start` equals `bot` -/
 def simpStartToBot {r : Regex α} (hr : r.CRegularAnchor)
@@ -35,7 +55,7 @@ def simpStartToBot {r : Regex α} (hr : r.CRegularAnchor)
   | unit c => ⟨_, unit c⟩
   | concat q r => ⟨_, concat q.simpStartToBot.2 r.simpStartToBot.2⟩
   | or q r => ⟨_, or q.simpStartToBot.2 r.simpStartToBot.2⟩
-  | star t r => ⟨_, star t r.simpStartToBot.2⟩
+  | star r => ⟨_, star r.simpStartToBot.2⟩
   | start => ⟨_, bot⟩ -- here!
   | end' => ⟨_, end'⟩
   | capture n r => ⟨_, capture n r.simpStartToBot.2⟩
@@ -46,7 +66,7 @@ def HasStart {r : Regex α} (hr : r.CRegularAnchor) := match hr with
   | unit _ => False
   | concat q r => q.HasStart ∨ r.HasStart
   | or q r => q.HasStart ∨ r.HasStart
-  | star _ r => r.HasStart
+  | star r => r.HasStart
   | start => True
   | end' => False
   | capture _ r => r.HasStart
@@ -83,20 +103,20 @@ def simpStartRec {motive : {r : Regex α} → r.CRegularAnchor → Sort*}
     (or_concat : {p q r : Regex α} → (hp : p.CRegularAnchor) →
       (hq : q.CRegularAnchor) → (hr : r.CRegularAnchor) →
       motive (concat hp hr) → motive (concat hq hr) → motive (concat (or hp hq) hr))
-    (star_concat : (t : StarType) → {q r : Regex α} →
+    (star_concat : {q r : Regex α} →
       (hq : q.CRegularAnchor) → (hr : r.CRegularAnchor) →
-      motive hq → motive hr → motive (concat (star t hq) hr))
+      motive hq → motive hr → motive (concat (star hq) hr))
     (start_concat : {r : Regex α} → (hr : r.CRegularAnchor) →
-      motive (concat .start hr))
+      motive hr → motive (concat .start hr))
     (end'_concat : {r : Regex α} → (hr : r.CRegularAnchor) →
-      motive (concat .end' hr))
+      motive hr → motive (concat .end' hr))
     (capture_concat : {n : ℕ} → {q r : Regex α} →
       (hq : q.CRegularAnchor) → (hr : r.CRegularAnchor) →
       motive (concat hq hr) → motive (concat (capture n hq) hr))
     (or : {q r : Regex α} → (hq : q.CRegularAnchor) → (hr : r.CRegularAnchor) →
       motive hq → motive hr → motive (or hq hr))
-    (star : (t : StarType) → {r : Regex α} → (hr : r.CRegularAnchor) →
-      motive hr → motive (star t hr))
+    (star : {r : Regex α} → (hr : r.CRegularAnchor) →
+      motive hr → motive (star hr))
     (start : motive start)
     (end' : motive end')
     (capture : (n : ℕ) → {r : Regex α} → (hr : r.CRegularAnchor) →
@@ -110,9 +130,66 @@ def simpStartRec {motive : {r : Regex α} → r.CRegularAnchor → Sort*}
   | .concat .bot r => bot_concat r
   | .concat .empty r => empty_concat r
       (simpStartRec bot empty unit bot_concat empty_concat unit_concat concat_concat
-      or_concat star_concat start_concat end'_concat capture_concat or star start end' capture r)
-  | .concat (.unit c) r => unit_concat r
-
+      or_concat star_concat start_concat end'_concat capture_concat or star start end' capture
+      r)
+  | .concat (.unit c) r => unit_concat c r
+  | .concat (.concat p q) r => concat_concat p q r
+      (simpStartRec bot empty unit bot_concat empty_concat unit_concat concat_concat
+      or_concat star_concat start_concat end'_concat capture_concat or star start end' capture
+      (.concat p (.concat q r)))
+  | .concat (.or p q) r => or_concat p q r
+      (simpStartRec bot empty unit bot_concat empty_concat unit_concat concat_concat
+      or_concat star_concat start_concat end'_concat capture_concat or star start end' capture
+      (.concat p r))
+      (simpStartRec bot empty unit bot_concat empty_concat unit_concat concat_concat
+      or_concat star_concat start_concat end'_concat capture_concat or star start end' capture
+      (.concat q r))
+  | .concat (.star q) r => star_concat q r
+      (simpStartRec bot empty unit bot_concat empty_concat unit_concat concat_concat
+      or_concat star_concat start_concat end'_concat capture_concat or star start end' capture
+      q) (simpStartRec bot empty unit bot_concat empty_concat unit_concat concat_concat
+      or_concat star_concat start_concat end'_concat capture_concat or star start end' capture
+      r)
+  | .concat .start r => start_concat r
+      (simpStartRec bot empty unit bot_concat empty_concat unit_concat concat_concat
+      or_concat star_concat start_concat end'_concat capture_concat or star start end' capture
+      r)
+  | .concat .end' r => end'_concat r
+      (simpStartRec bot empty unit bot_concat empty_concat unit_concat concat_concat
+      or_concat star_concat start_concat end'_concat capture_concat or star start end' capture
+      r)
+  | .concat (.capture n q) r => capture_concat q r
+      (simpStartRec bot empty unit bot_concat empty_concat unit_concat concat_concat
+      or_concat star_concat start_concat end'_concat capture_concat or star start end' capture
+      (.concat q r))
+  | .or q r => or q r
+      (simpStartRec bot empty unit bot_concat empty_concat unit_concat concat_concat
+      or_concat star_concat start_concat end'_concat capture_concat or star start end' capture
+      q) (simpStartRec bot empty unit bot_concat empty_concat unit_concat concat_concat
+      or_concat star_concat start_concat end'_concat capture_concat or star start end' capture
+      r)
+  | .star r => star r
+      (simpStartRec bot empty unit bot_concat empty_concat unit_concat concat_concat
+      or_concat star_concat start_concat end'_concat capture_concat or star start end' capture
+      r)
+  | .start => start
+  | .end' => end'
+  | .capture n r => capture n r
+      (simpStartRec bot empty unit bot_concat empty_concat unit_concat concat_concat
+      or_concat star_concat start_concat end'_concat capture_concat or star start end' capture
+      r)
+termination_by (hr.regex.depth, hr.simpStartSize)
+decreasing_by
+  rotate_left 1
+  · simp only [regex_eq, depth, simpStartSize, Prod.lex_def, Order.lt_add_one_iff,
+      Order.add_one_le_iff, Nat.add_right_cancel_iff]
+    right
+    constructor
+    · rw [Nat.add_right_comm]; simp [Nat.add_assoc]
+    split
+    · expose_names; simp at heq; simp [heq.1, depth]
+    · exact Nat.zero_le _
+  all_goals simp [Prod.lex_def, simpStartSize, depth] <;> try linarith
 
 /-- Get a regex that's language-equivalent to this regex, but doesn't
 have any start anchors. -/
@@ -127,13 +204,13 @@ def simpStart {r : Regex α} (hr : r.CRegularAnchor)
   | concat (unit _) r => ⟨_, r.simpStartToBot.2⟩
   | concat (concat p q) r => (concat p (concat q r)).simpStart
   | concat (or p q) r => ⟨_, or (concat p r).simpStart.2 (concat q r).simpStart.2⟩
-  | concat (star t q) r => ⟨_, or r.simpStart.2 (concat q.simpStart.2
-      (concat (star t q.simpStartToBot.2) r.simpStartToBot.2))⟩
+  | concat (star q) r => ⟨_, or r.simpStart.2 (concat q.simpStart.2
+      (concat (star q.simpStartToBot.2) r.simpStartToBot.2))⟩
   | concat start r => ⟨_, r.simpStart.2⟩
-  | concat end' r => ⟨_, r.simpStart.2⟩
+  | concat end' r => ⟨_, concat end' r.simpStart.2⟩
   | concat (capture n q) r => (concat q r).simpStart
   | or q r => ⟨_, or q.simpStart.2 r.simpStart.2⟩
-  | star t r => ⟨_, or empty (concat r.simpStart.2 (star t r.simpStartToBot.2))⟩
+  | star r => ⟨_, or empty (concat r.simpStart.2 (star r.simpStartToBot.2))⟩
   | start => ⟨_, empty⟩
   | end' => ⟨_, end'⟩
   | capture n r => ⟨_, capture n r.simpStart.2⟩
@@ -156,14 +233,34 @@ theorem simpStartToBot_noStart {r : Regex α} (hr : r.CRegularAnchor)
     : ¬hr.simpStartToBot.2.HasStart := by
   induction hr <;> simp [simpStartToBot, HasStart, *]
 
-/-- `simpStartToBot` removes all start anchors -/
+omit deq in
+/-- `simpStart` removes all start anchors -/
 theorem simpStart_noStart {r : Regex α} (hr : r.CRegularAnchor)
     : ¬hr.simpStart.2.HasStart := by
   induction hr using simpStartRec
-  --induction (hr.regex.depth, hr.simpStartSize)
-  --induction hr <;> try rw [simpStart.eq_def]; simp [HasStart, *]
-  --case concat q r qind rind =>
-  --  cases q
+  all_goals rw [simpStart.eq_def]; simp [HasStart, simpStartToBot_noStart, *]
+
+/-- `simpStart` produces an equivalent language -/
+theorem languageEquiv_simpStart {r : Regex α} (hr : r.CRegularAnchor)
+    : r ≃ˡᵃ hr.simpStart.1 := by
+  refine ⟨hr.terminatesEquiv hr.simpStart.2, ?_⟩
+  induction hr using simpStartRec
+  case bot | empty | unit _ | end' => simp [simpStart]
+  case bot_concat r => simp [languageEquiv_bot_concat.2, simpStart]
+  case empty_concat r => simp [languageEquiv_empty_concat.2, simpStart, r]
+  case unit_concat c r => sorry
+  case concat_concat p q r => simp [languageEquiv_concat_assoc.2, simpStart, r]
+  case or_concat p q r => simp [languageEquiv_or_concat.2, simpStart, isMatch_or, q, r]
+  case star_concat q r => sorry
+  case start_concat r rind => simp [(languageEquiv_start_concat
+    fun w s cap _ ↦ r.allTerminates w s cap).2, simpStart, rind]
+  case end'_concat r rind => simp [(languageEquiv_end'_concat ⟨
+    r.terminatesEquiv r.simpStart.2, rind⟩).2, simpStart]
+  case capture_concat n q r => sorry
+  case or q r => simp [simpStart, isMatch_or, q, r]
+  case star r => simp [simpStart]; sorry
+  case start => simp [simpStart, isMatch_start, isMatch_empty]
+  case capture n r => simp [simpStart, isMatch_capture, r]
 
 end CRegularAnchor
 
